core/Peo.v
@@ -2,6 +2,7 @@ From Ssara.Core Require Import RegClass.
 From Ssara.Core Require Import RegSet.
 From Ssara.Core Require Import InterfGraph.
 From Ssara.Core Require Import Dict.
+From Ssara.Core Require Import Utils.
 From Stdlib Require Import ZArith.
 From Stdlib Require Import Lists.List.
 From Stdlib Require Import Bool.
@@ -10,69 +11,44 @@ From Ssara.Core Require Import RegVregInstance.
 Existing Instance reg_vreg_instance.
 
 (* Check whether regs are neighbors of r *)
-Definition are_neighbors (r : reg) (regs : list reg) (g : ig) : bool :=
+Definition are_neighbors (g : ig) (r : reg) (regs : list reg) : bool :=
   regs_mem r (dict_keys g) &&
-  fold_left
-    (fun b r' =>
-      b &&
-      ((r =? r') ||
-        regs_mem r' (ig_map g r)))
-    regs
-    true
+  conjunction (fun r' => (r =? r') || regs_mem r' (dict_map g r)) regs
 .
 
-Definition is_simplicial (r : reg) (g : ig) : bool :=
-  let regs := ig_map g r in
+(* Check whether the neighbors of r are a clique *)
+Definition is_simplicial (g : ig) (r : reg) : bool :=
+  let regs := dict_map g r in
   regs_mem r (dict_keys g) &&
-  fold_left (* Check whether the neighbor set of r is a clique *)
-    (fun b r =>
-      b &&
-      are_neighbors r regs g
-    )
-    regs
-    true
-.
-
-Fixpoint find_next_aux (regs : list reg) (g : ig) : option reg :=
-  match regs with
-  | nil => None
-  | r :: rs =>
-    if is_simplicial r g then Some r else find_next_aux rs g
-  end
+  conjunction (fun r' => are_neighbors g r' regs) regs
 .
 
 Definition find_next (g : ig) : option reg :=
-  find_next_aux (dict_keys g) g
+  find (is_simplicial g) (dict_keys g)
 . 
 
-Lemma find_next_mem :
+Lemma find_next_in :
   forall (g : ig) (n : reg), find_next g = Some n -> In n (dict_keys g)
 .
 Proof.
-  intros g n H. unfold find_next in H. generalize dependent n.
-  induction (dict_keys g) as [|r rs IH].
-  - intros n'. simpl. congruence.
-  - intros n'. simpl.
-    destruct (is_simplicial r g).
-    + intros H. injection H. intro H0. left. assumption.
-    + intros H. apply IH in H. right. assumption.
+  intros g n. unfold find_next. apply find_some.
 Qed.
 
 From Stdlib Require Import FunInd.
 From Stdlib Require Import Recdef.
 
-Function eliminate (g : ig) {measure dict_size g} : ig * list vreg :=
+Function eliminate (g : ig) {measure dict_size g} : list vreg :=
   match find_next g with
   | Some next =>
     let g' := ig_remove_node g next in
-    let (g'', peo) := eliminate g' in
-    (g'', next :: peo)
-  | None => (g, nil)
+    let peo := eliminate g' in
+    next :: peo
+  | None => nil
   end
 .
 Proof.
   intros g n H.
-  apply find_next_mem in H.
+  apply find_next_in in H.
   apply dict_size_decrease.
   assumption.
 Qed.
