core/InterfGraph.v
@@ -18,8 +18,6 @@ Instance dict_ig_instance : DictClass := {|
   key_eq_dec := Nat.eq_dec;
 |}.
 Definition ig : Type := dict.
-Definition ig_empty : ig := dict_empty.
-Definition ig_map : ig -> reg -> set reg := dict_map.
 
 Definition ig_update_edge (f : reg -> set reg -> set reg) (g : ig) (r : reg) (r' : reg) : ig :=
   let regs  := dict_map g r in
@@ -79,40 +77,6 @@ Fixpoint ig_insert_edges (g : ig) (r : reg) (regs : list reg) : ig :=
   end
 .
 
-(* Definition ig : Type := set reg * set (reg * reg).
-Definition ig_empty : ig := (nil, nil).
-Definition ig_map (g : ig) (r : reg) : list reg :=
-  let e := filter (fun '(r', _) => reg_eqb r r') (snd g) in
-  map fst e
-.
-
-Lemma edge_eq_dec : forall e e' : (reg * reg), {e = e'} + {e <> e'}.
-Proof.
-  decide equality.
-  - apply reg_eq_dec.
-  - apply reg_eq_dec.
-Qed.
-
-Definition ig_insert_edge (g : ig) (r : reg) (r' : reg) : ig :=
-  let (v, e) := g in
-  (regs_add r' (regs_add r v),
-  set_add edge_eq_dec (r, r') (set_add edge_eq_dec (r, r') e))
-.
-
-Definition ig_insert_node (g : ig) (r : reg) : ig :=
-  let (v, e) := g in (regs_add r v, e)
-.
-
-Fixpoint ig_insert_edges (g : ig) (r : reg) (rs : list reg) : ig :=
-  match rs with
-  | nil => g
-  | r' :: tl =>
-    if r =? r'
-    then ig_insert_edges (ig_insert_node g r) r tl
-    else ig_insert_edges (ig_insert_edge g r r') r tl
-  end
-. *)
-
 Definition ig_insert_clique (g : ig) (regs : list reg) : ig :=
   fold_left
     (fun g_acc r => (ig_insert_edges g_acc r regs))
@@ -141,7 +105,7 @@ Definition get_ig (pi : programinfo) : ig :=
       end
     )
     ls
-    ig_empty
+    dict_empty
 .
 
 (*
@@ -199,7 +163,7 @@ Module Example1.
   Compute
     let '(pi, _) := analyze_program example_block_1 fuel in
     let g := get_ig pi in
-    g
+    dict_list g
   .
 End Example1.
 
@@ -243,7 +207,7 @@ Module Example2.
   Compute
     let '(pi, _) := analyze_program example_block_1 fuel in
     let g := get_ig pi in
-    g
+    dict_list g
   .
 End Example2.
 
@@ -288,6 +252,6 @@ Module Example3.
   Compute
     let '(pi, _) := analyze_program example_block_1 fuel in
     let g := get_ig pi in
-    g
+    dict_list g
   .
 End Example3.
