core/Utils.v
@@ -1,6 +1,13 @@
+From Stdlib Require Import Lists.List.
+From Stdlib Require Import Bool.
+
 Definition option_to_list {A : Type} (x : option A) : list A :=
   match x with
   | Some x' => x' :: nil
   | None => nil
   end
+.
+
+Definition conjunction {A : Type} (f : A -> bool) (l : list A) : bool :=
+  fold_left (fun b x => b && f x) l true
 .
