extract/Extract.v
@@ -1,9 +1,10 @@
-From Ssara.Core Require Import Syntax.
 From Ssara.Core Require Import Vm.
-From Ssara.Core Require Import RegAlloc.
+From Ssara.Core Require Import Syntax.
 From Ssara.Core Require Import LivenessInfo.
 From Ssara.Core Require Import InterfGraph.
 From Ssara.Core Require Import Peo.
+From Ssara.Core Require Import RegAlloc.
+From Ssara.Core Require Import Destruct.
 From Ssara.Core Require Import RegPregInstance.
 From Ssara.Core Require Import RegVregInstance.
 
@@ -31,5 +32,5 @@ Extraction "ssara.ml"
   Peo.eliminate
   RegAlloc.get_coloring
   RegAlloc.color_program
-  RegAlloc.Example1.example_block_1
+  (* RegAlloc.Example1.example_block_1 *)
 .
